CoqOfRust/revm/revm_interpreter/instructions/links/bitwise.v
@@ -1,0 +1,79 @@
+Require Import CoqOfRust.CoqOfRust.
+Require Import CoqOfRust.links.lib.
+Require Import CoqOfRust.links.M.
+Require Import revm.revm_context_interface.links.host.
+Require revm.links.dependencies.
+Import revm.links.dependencies.ruint.
+Require Import revm.revm_interpreter.links.gas.
+Require Import revm.revm_interpreter.links.interpreter.
+Require Import revm.revm_interpreter.links.interpreter_types.
+Require Import revm.revm_interpreter.instructions.bitwise.
+
+Import Run.
+(*
+pub fn add<WIRE: InterpreterTypes, H: Host + ?Sized>(
+    interpreter: &mut Interpreter<WIRE>,
+    _host: &mut H,
+)
+
+pub fn lt<WIRE: InterpreterTypes, H: Host + ?Sized>(
+    interpreter: &mut Interpreter<WIRE>,
+    _host: &mut H,
+)
+*)
+
+Definition run_lt
+    {WIRE H : Set} `{Link WIRE} `{Link H}
+    {WIRE_types : InterpreterTypes.Types.t} `{InterpreterTypes.Types.AreLinks WIRE_types}
+    (run_InterpreterTypes_for_WIRE : InterpreterTypes.Run WIRE WIRE_types)
+    (interpreter : Ref.t Pointer.Kind.MutRef (Interpreter.t WIRE WIRE_types))
+    (_host : Ref.t Pointer.Kind.MutRef H) :
+  {{
+    instructions.bitwise.lt [] [ Φ WIRE; Φ H ] [ φ interpreter; φ _host ] 🔽
+    unit
+  }}.
+Proof.
+  run_symbolic.
+  eapply Run.Rewrite. {
+    repeat erewrite IsTraitAssociatedType_eq by apply run_InterpreterTypes_for_WIRE.
+    reflexivity.
+  }
+  run_symbolic_let. {
+    run_symbolic.
+    destruct run_InterpreterTypes_for_WIRE.
+    destruct run_LoopControl_for_Control.
+    destruct gas as [gas [H_gas run_gas]].
+    destruct set_instruction_result as [set_instruction_result [H_set_instruction_result run_set_instruction_result]].
+    run_symbolic.
+    run_symbolic_closure. {
+      apply Impl_Gas.run_record_cost.
+    }
+    intros []; run_symbolic.
+    run_symbolic_are_equal_bool; run_symbolic.
+  }
+  intros [|[]]; run_symbolic.
+  destruct run_InterpreterTypes_for_WIRE.
+  destruct run_StackTrait_for_Stack.
+  destruct popn_top as [popn_top [H_popn_top run_popn_top]].
+  run_symbolic.
+  run_symbolic_let. {
+    run_symbolic.
+    eapply Run.CallPrimitiveGetTraitMethod.
+    { eapply IsTraitMethod.Defined.
+       - specialize (Impl_PartialOrd_for_Uint.Implements
+       (Value.Integer IntegerKind.Usize 256)
+       (Value.Integer IntegerKind.Usize 4)).
+       intros.
+       unfold Impl_PartialOrd_for_Uint.Self in H3.
+       apply H3 with (trait_tys := [Ty.apply (Ty.path "ruint::Uint")
+        [Value.Integer IntegerKind.Usize 256;
+         Value.Integer IntegerKind.Usize 4] []]).
+      - simpl.
+        reflexivity.
+    }
+    run_symbolic.
+    
+  }
+  intros [|[]]; run_symbolic.
+
+
